---
layout: clrs-solution
title: "Exercise 28.1-1"
---

> Solve the equation $$\begin{pmatrix} 1 & 0 & 0 \\ 4 & 1 & 0 \\ -6 & 5 & 1 \end{pmatrix} \begin{pmatrix} x_1 \\ x_2 \\ x_3 \end{pmatrix} = \begin{pmatrix} 3 \\ 14 \\ -7 \end{pmatrix}$$ by using forward substitution.

This equation is already setup for us to apply forward substition because the first matrix is a lower triangular matrix and the second contains only unknown variables. So we may simply solve the three different subequations sequentially:

$$ x_1 = 3$$

$$
\begin{align*}
4x_1 + x_2 &= 14 \\
12 + x_2 &= 14 \\
x_2 &= 2
\end{align*}
$$

$$
\begin{align*}
-6x_1 + 5x_2 + x_3 &= -7 \\
-18 + 10 + x_3 &= -7 \\
x_3 &= 1 \\
\end{align*}
$$

So we have:

$$ \begin{pmatrix} x_1 \\ x_2 \\ x_3 \end{pmatrix} = \begin{pmatrix} 3 \\ 2 \\ 1 \end{pmatrix}$$
