---
layout: clrs-solution
title: "Exercise 15.1-1"
---

> Show that equation (15.4) follows from equation (15.3) and the initial condition $$T(0) = 1$$.

For reference, equation 15.3 states:

$$T(n) = 1 + \sum^{n-1}_{j=0} T(j)$$

and we want to prove the claim of equation 15.4 that $$T(n) = 2^n$$. Suppose $$n \ge 1$$ and consider $$T(n-1)$$:

$$T(n-1) = 1 + \sum^{n-2}_{j=0} T(j)$$

If we subtract $$T(n-1)$$ from $$T(n)$$, everything cancels out except for the final term of the summation which is present in $$T(n)$$ but not in $$T(n-1)$$:

$$
\begin{align*}
T(n) - T(n-1) &= T(n - 1) \\
T(n) &= 2T(n-1)
\end{align*}
$$

The pattern is easy to observe:

$$ T(1) = 2T(0) = 2 \cdot 1 = 2 $$

$$ T(2) = 2T(1) = 2 \cdot 2 = 4 $$

$$ T(3) = 2T(2) = 2 \cdot 4 = 8 $$

$$ \vdots $$

$$ T(n) = 2^n$$

From another angle, let's assume $$T(j) = 2^j$$ for all $$0 \le j \le n-1$$. Then by (A.5) we have:

$$ \sum^{n-1}_{j=0} T(j) = \sum^{n-1}_{j=0} 2^j = \frac{2^{n+1-1} - 1}{2-1} = 2^n - 1 $$

And so:

$$ T(n) = 1 + \sum^{n-1}\_{j=0} T(j) = 1 + (2^n - 1) = 2^n$$

Since $$2^0 = 1$$ the base case of T(0) = 1 holds and therefore this claim is also proved by induction.
