---
layout: clrs-solution
title:  "Exercise 3.1-2"
---
>Show that for any real constants $$a$$ and $$b$$, where $$b > 0$$,
>
>$$(n + a)^b = \Theta(n^b)$$.



By the Binomial Theorem, $$(n + a)^b =  \sum\limits_{k=0}^{b}\binom{b}{k}n^{b-k}a{k} = C_{0}^{b}n^{b}a^0 + C_{1}^{b}n^{b-1}a^1 + \cdots + C_{b}^{b}n^{0}a^b$$. In order to simplify further calculations, we want to restrict $$n + a$$ to be non-negative which we can do by setting $$n_0 \geq \lvert a \rvert$$. With $$n + a \geq 0$$ we know that:

$$0 \leq C_{0}^{b}n^b \leq C_{0}^{b}n^{b}a^0 + C_{1}^{b}n^{b-1}a^1 + \cdots + C_{b}^{b}n^{0}a^b$$

We are interested in values of $$n$$ such that $$n \geq n_0$$, and since we know $$n_0$$ is positive, we can use the fact that $$C_{0}^{b}n^{b}a^0 + C_{1}^{b}n^{b-1}a^1 + \cdots + C_{b}^{b}n^{0}a^b \leq (C_{0}^{b} + C_{1}^{b} + \cdots + C_{b}^{b})n^b$$ to construct another step in our inequality:

$$0 \leq C_{0}^{b}n^b \leq C_{0}^{b}n^{b}a^0 + C_{1}^{b}n^{b-1}a^1 + \cdots + C_{b}^{b}n^{0}a^b \leq (C_{0}^{b} + C_{1}^{b} + \cdots + C_{b}^{b})n^b$$

Which is the definition of $$\Theta(n^b)$$ with $$c_1 = C_{0}^{b} = 1$$, $$c_2 = C_{0}^{b} + C_{1}^{b} + \cdots + C_{b}^{b}$$ and $$n_0 \geq \lvert a \rvert$$.