---
layout: clrs-solution
title:  "Exercise 3.2-2"
---
>Prove $$a^{\log_b{c}} = c^{\log_b{a}}$$ where $$b \neq 1$$.

To start we have:

$$a^{\log_bc}$$

Using the identity $$\log_b{a} = \frac{\log_c{a}}{\log_c{b}}$$ we can obtain:

$$a^{\log_bc} = a^{\frac{\log_a{c}}{\log_a{b}}}$$

Next we can use routine exponential identities to rearrange our terms:

$$a^{\log_bc} = a^{\frac{\log_a{c}}{\log_a{b}}} = (a^{\log_a{c}})^{\frac{1}{\log_a{b}}}$$

Based on the identity $$a = b^{\log_b{a}}$$:

$$a^{\log_bc} = a^{\frac{\log_a{c}}{\log_a{b}}} = (a^{\log_a{c}})^{\frac{1}{\log_a{b}}} = c^{\frac{1}{\log_a{b}}}$$

Lastly we use the identity $$\log_b{a} = \frac{1}{log_a{b}}$$ to complete the proof:

$$a^{\log_bc} = a^{\frac{\log_a{c}}{\log_a{b}}} = (a^{\log_a{c}})^{\frac{1}{\log_a{b}}} = c^{\frac{1}{\log_a{b}}} = c^{\log_b{a}}$$