---
layout: clrs-solution
title:  "Exercise 3.2-7"
---
>Prove by induction that the $$i$$th Fibonacci number satisfies the equality
>
> $$F_i = \frac{\phi^i - \hat{\phi^i}}{\sqrt{5}}$$,
>
> where $$\phi$$ is the golden ratio and $$\hat{\phi}$$ is its conjugate.

For our base case, we need two values of $$F$$:

$$F_0 = \frac{\phi^0 - \hat{\phi^0}}{\sqrt{5}} = \frac{1 - 1}{\sqrt{5}} = 0$$

$$F_1 = \frac{\phi^1 - \hat{\phi^1}}{\sqrt{5}} = \frac{\frac{1 + \sqrt{5}}{2} - \frac{1 - \sqrt{5}}{2}}{\sqrt{5}} = \frac{1 + \sqrt{5} - 1 + \sqrt{5}}{2\sqrt{5}} = \frac{2\sqrt{5}}{2\sqrt{5}} = 1$$

For the inductive step, recall that $$F_i = F_{i-1} + F_{i-2}$$ for $$ i \geq 2 $$:

$$\begin{equation}
\begin{split}
F_i & = \frac{\phi^{i-1} - \hat{\phi}{}^{i-1}}{\sqrt{5}} + \frac{\phi^{i-2} - \hat{\phi}{}^{i-2}}{\sqrt{5}} \\
& = \frac{\phi^{i-1} + \phi^{i-2} - \hat{\phi}{}^{i-1} - \hat{\phi}{}^{i-2}}{\sqrt{5}} \\
& = \frac{\phi^{i-2}(\phi + 1) - \hat{\phi}{}^{i-2}(\hat{\phi} + 1)}{\sqrt{5}} \\
& = \frac{\phi^{i-2}\phi^2  - \hat{\phi}{}^{i-2}\hat{\phi}{}^{2}}{\sqrt{5}} \\
& = \frac{\phi^i  - \hat{\phi}{}^i}{\sqrt{5}} \\
\end{split}
\end{equation}$$