---
layout: clrs-solution
title:  "Exercise 3.2-8"
---
>Show that $$k \ln k = \Theta(n) \implies k = \Theta \left( \frac{n}{\ln n} \right)$$.

Via symmetry, we have $$f(n) = \Theta(g(n)) \iff g(n) = \Theta(f(n))$$ so $$ k \ln k = \Theta(n) \implies n = \Theta(k \ln k)$$.

$$\begin{equation}
\begin{split}
\ln n & = \Theta ( \ln ( k \ln k)) \\
& = \Theta( \ln k + \ln \ln k) \\
& = \Theta ( \ln k) 
\end{split}
\end{equation}$$

Since we now have the values of both $$\Theta(n)$$ and $$\Theta(\ln n)$$ which via symmetry give us $$n$$ and $$\ln n$$:

$$\begin{equation}
\begin{split}
\frac{n}{\ln n} & = \frac{\Theta(k \ln k)}{\Theta ( \ln k)} \\
& = \Theta \left( \frac{k \ln k}{\ln k} \right) \\
& = \Theta(k)
\end{split}
\end{equation}$$

Therefore with the help of symmetry one last time, we conclude that $$k = \Theta \left( \frac{n}{\ln n} \right)$$.