---
layout: clrs-solution
title:  "Exercise 7.2-1"
---
>Use the substitution method to prove that the recurrence $$T(n) = T(n-1) + \Theta(n)$$ has the solution $$T(n) = \Theta(n^2)$$, as claimed at the beginning of Section 7.2.

We guess $$T(n) \leq cn^2$$ for some constant $$c > 0$$. Furthermore, we will represent $$\Theta(n)$$ as $$dn$$. Substituting these into the recurrence yields

$$\begin{split}
T(n) &\leq T(n-1) + dn \\
&= c(n-1)^2 + dn \\
&= cn^2 -2cn + c + dn \\
&\leq cn^2 \\
\end{split}$$

where the last step holds for when $$2c > d$$ and $$c \geq \frac{dn}{2n-1}$$.