---
layout: clrs-solution
title:  "Exercise 4.3-2"
---
>Show that the solution of $$T(n) = T(\lceil n/2 \rceil) + n$$ is $$O(\lg n)$$.

In order to use the substitution method, we guess that the solution is $$O(\lg n)$$ and must prove that $$T(n) \leq c \lg n$$ for some $$c > 0$$. We assume that this bound holds for all positive $$m < n$$ such as $$m = \lceil n/2 \rceil$$ (for sufficient values of $$n$$):

$$T(\lceil n/2 \rceil) \leq c \lg( \lceil n/2 \rceil) + 1$$

Substituting into the recurrence yields

$$\begin{split}
T(n) & \leq c \lg (\lceil n/2 \rceil) + 1 \\
& = c \lg \left( \frac{n}{2} + 1 \right) + 1 \\
& = c \lg \left( \frac{n + 2}{2} \right) + 1 \\
& = c(\lg ( n + 2) - \lg(2)) + 1 \\
& = c\lg(n+2) - c + 1 \\
& \leq \lg n
\end{split}$$

Unfortunately, there are no values of $$c$$ for which the last step holds. Given the form of our final step, let us modify our original guess slightly to be $$T(n) \leq c \lg(n-d)$$ for some constant $$d$$. We make the same assumption that this bound holds for all positive $$m < n$$ such as $$m = \lceil n/2 \rceil$$ (for sufficient values of $$n$$):

$$T(\lceil n/2 \rceil) \leq c \lg( \lceil n/2 \rceil - d) + 1$$

Substituting into the recurrence yields

$$\begin{split}
T(n) & \leq c \lg (\lceil n/2 \rceil - d) + 1 \\
& = c \lg \left( \frac{n}{2} - d + 1 \right) + 1 \\
& = c \lg \left( \frac{n -2d + 2}{2} \right) + 1 \\
& = c(\lg ( n -2d + 2) - \lg(2)) + 1 \ \ \ ( \text{let} \ d = 2 ) \\
& = c\lg(n - 2) - c + 1 \ \ \ ( \text{let} \ c = 1 )  \\
& = \lg(n - 2) \\
& \leq \lg n
\end{split}$$

This last step holds for $$c = 1$$, $$d = 2$$ and all $$n > 2$$.