---
layout: clrs-solution
title:  "Exercise 4.3-9"
---
>Solve the recurrence $$T(n) = 3T(\sqrt{n}) + \log n$$ by making a change of variables. Your solution should be asymptotically tight. Do not worry about whether values are integral.

Let $$m = \lg n$$. Then we have $$T(2^m) = 3T(2^{m/2}) + m$$ and we can rename $$S(m) = T(2^m)$$ to produce the new recurrence $$S(m) = 3S(m/2) + m$$. We can use the master method on this recurrence and so we have $$a = 3$$, $$b = 2$$ and $$f(m) = m$$.

Case 1 applies since $$f(m) = O(m^{\log_2 3 - \epsilon}) = O(m^{\log_2 2}) = O(m)$$, and thus the solution to the recurrence is $$S(m) = \Theta(m^{\log_2 3}) = O(m^{\lg 3})$$.

In order to show asymptotic tightnes, let's confirm that $$S(m) = O(m^{\lg 3})$$ by guessing that $$S(m) \leq cm^{\lg 3} - bm$$. Substituting this into the recurrence yields

$$\begin{split}
S(m) & \leq 3 \left( c \left( \frac{m}{2}\right)^{\lg 3} - b \frac{m}{2}\right) + m \\
& = 3 \left( \frac{cm^{\lg 3}}{2^{\lg 3}} - \frac{bm}{2} \right) + m \\
& = \frac{3cm^{\lg 3}}{3} - \frac{3bm}{2} + m \\
& = cm^{\lg 3} - \frac{3bm}{2} + m \\
& \leq cm^{\lg 3} - bm \\
\end{split}$$

Where the last step holds for $$b \geq 2$$. Next, let's confirm that $$S(m) = \Omega(m^{\lg 3})$$ by guessing that $$S(m) \leq cm^{\lg 3}$$. Substituting this into the recurrence yields

$$\begin{split}
S(m) & \geq 3c \left( \frac{m}{2} \right)^{\lg 3} + m \\
& = 3c \frac{m^{\lg 3}}{3} + m \\
& = cm^{\lg 3} + m \\
& \geq cm^{\lg 3} \\
\end{split}$$

Where the last step trivially holds. The combination of $$S(m) = O(m^{\lg 3})$$ and $$S(m) = \Omega(m^{\lg 3})$$ means that our solution is asymptotically tight, or in other words $$S(m) = \Theta(m^{\lg 3})$$.

Lastly, changing back from $$S(m)$$ to $$T(n)$$ we obtain

$$T(n) = T(2^m) = S(m) = \Theta(m^{\lg 3}) = \Theta(\lg^{\lg 3} n)$$