---
layout: clrs-solution
title:  "Exercise 4.3-1"
---
>Show that the solution of $$T(n) = T(n-1) + n $$ is $$O(n^2)$$.

In order to use the substitution method, we guess that the solution is $$O(n^2)$$ and must prove that $$T(n) \leq cn^2$$ for some $$c > 0$$. We assume that this bound holds for all positive $$m < n$$ such as $$m = n - 1$$:

 $$T(n - 1) \leq c(n-1)^2$$

Substituting into the recurrence yields

$$\begin{split}
T(n) & \leq c(n-1)^2 + n \\
& = cn^2 -2cn + n + c \ \ \ ( \text{let} \ c = 1 ) \\
& = n^2 -2n + n + 1 \\
& = n^2 -n + 1 \\
& \leq n^2 \\
\end{split}$$

We say that the last step holds for $$n \geq 1$$ and $$c = 1$$ as noted above. To be clear, the last step is claiming $$ n^2 -n + 1 \leq n^2 \ \forall \ n \geq 1$$ which wasn't immediately clear to me with this notation for the substitution method.