---
layout: clrs-solution
title:  "Exercise 4.3-7"
---
>Using the master method in Section 4.5, you can show that the solution to the recurrence $$T(n) = 4T(n/3) + n$$ is $$T(n) = \Theta(n^{\log_3 4})$$. Show that a substitution proof with the assumption $$T(n) \leq cn^{\log_3 4}$$ fails. Then show how to subtract off a lower-order term to make a substitution proof work.

We start by substituting our doomed guess of $$T(n) \leq cn^{\log_{3}4}$$ into the recurrence

$$\begin{split}
T(n) & \leq 4c \left(\frac{n}{3}\right)^{\log_{3}4} + n \\
& = 4c \left(\frac{n^{\log_{3}4}}{3^{\log_{3}4}}\right) + n \\
& = 4c \left(\frac{n^{\log_{3}4}}{4}\right) + n \\
& = cn^{\log_{3}4} + n \\
\end{split}$$

Which we cannot proceed further from. Next, let us modify our guess to subtract a lower-order term: $$T(n) \leq cn^{\log_{3}4} - bn$$. Substituting this new guess into the recurrence:

$$\begin{split}
T(n) & \leq 4 \left(c \left(\frac{n}{3}\right)^{\log_{3}4} - b \frac{n}{3} \right) + n \\
& = 4c \frac{n^{\log_{3}4}}{4} - \frac{4}{3}bn + n \\
& \leq cn^{\log_{3}4} - bn \\
\end{split}$$

Where the last step holds for $$b \geq 3$$.