---
layout: clrs-solution
title:  "Exercise 4.4-6"
---
>Argue that the solution to the recurrence $$T(n) = T(n/3) + T(2n/3) + cn$$, where $$c$$ is a constant, is $$\Omega(n \lg n)$$ by appealing to a recursion tree.

The recurrence $$T(n) = T(n/3) + T(2n/3) + cn$$ has the following recursion tree (Note that this is identical to figure 4.6 in the text)

![4.4-6 Recursion Tree]({{ '/assets/img/4-4-6.png' | prepend: site.baseurl }}){:class="latex-img"}

The shortes simple path from the root to a leaf is $$n \rightarrow (1/3)n \rightarrow (1/3)^2n \rightarrow \cdots \rightarrow 1$$. Since $$(1/3)^kn = 1$$ when $$k = \log_{3}n$$, this path has length $$\log_{3}n$$. Thus the cost of the algorith is

$$cn(\log_{3}n + 1) \geq cn \log_{3} n = \frac{c}{\log_{3}}n \log n = \Omega(n \log n)$$