---
layout: clrs-solution
title:  "Exercise 4.4-5"
---
>Use a recursion tree to determine a good asymptotic upper bound on the recurrence $$T(n) = T(n-1) + T(n/2) + n$$. Use the substitution method to verify your answer.

The recurrence $$T(n) = T(n-1) + T(n/2) + n$$ has the following recursion tree (Note however that this tree is not full as one path depletes $$n$$ much quicker than the other)

![4.4-5 Recursion Tree]({{ '/assets/img/4-4-5.png' | prepend: site.baseurl }}){:class="latex-img"}

Summing the cost of the longest simple path from the root to a leaf is

$$\begin{split}
\sum\limits_{i=0}^{n}c(n-i) & = c\sum\limits_{i=0}^{n}i \\
& = c \frac{n(n+1)}{2} \\
& = c \frac{n^2}{2} + \frac{c}{2} \\
& = O(n^2) \\
\end{split}$$

This informs our guess for a lower bound: $$T(n) \geq cn^2$$. Substituting this into the recurrence yields

$$\begin{split}
T(n) & \geq c(n-1)^2 + c\left(\frac{n}{2}\right)^2 + n \\
& = cn^2 - 2cn + 1 + \frac{cn^2}{4} + n \\
& = \frac{5}{4}cn^2 - 2cn + n + 1 \\
& \geq cn^2 \\
\end{split}$$

Where the last step holds for all $$c \geq 1$$. Thus we have $$T(n) = \Omega(n^2)$$.

Our recursion tree doesn't provide any obvious insight into an upper bound. But consider a similar recurrence 

$$S(n) = 2T(n-1) + n$$

which is similar to $$T(n)$$ but is more costly. We know that $$S(n) = O(2^n)$$ so a reasonable guess for our unique recurrence $$T(n)$$ would be $$T(n) \leq c2^n - bn$$. Substituting this into the recurrence yields

$$\begin{split}
T(n) & \leq 2(c2^{n-1} - b(n - 1)) + n \\
& = c2^n - 2bn + 2b + n \\
& = c2^n - bn - n(b - 1) + 2b \\
& \leq c2^n - bn \\
\end{split}$$

Where the last step holds for $$b \geq 3$$. Therefore we have $$T(n) = O(2^n)$$.

The following LaTeX code was used to generate the above recursion tree:

{% highlight latex %}
\documentclass[12pt]{article}
\usepackage{forest}
\usepackage{tikz-qtree}
\begin{document}

\begin{figure}
\begin{minipage}[b]{0.5\linewidth}
\centering
\begin{tikzpicture}[scale=.75,sibling distance=0pt]
\Tree [.$cn$ 
        [.$c(n-1)$ 
          [.$c(n-2)$ 
            [.$c(n-3)$ 
              [.$\vdots$ ] ] 
            [.$c\frac{(n-2)}{2}$ 
              [.$\vdots$ ] ] ] 
          [.$c\frac{(n-1)}{2}$ 
            [.$c\left(\frac{(n-1)}{2}-1\right)$ 
              [.$\vdots$ ] ] 
            [.$c\frac{(n-1)}{4}$ 
              [.$\vdots$ ] ] ] ]
        [.$c\frac{n}{2}$ 
          [.$c\left(\frac{n}{2}-1\right)$ 
            [.$c\left(\frac{n}{2}-2\right)$ 
              [.$\vdots$ ] ]
            [.$\frac{c\left(\frac{n}{2}-1\right)}{2}$ 
              [.$\vdots$ ] ] ]
          [.$c\frac{n}{4}$ 
            [.$c\left(\frac{n}{4}-1\right)$ 
              [.$\vdots$ ] ]
            [.$c\frac{n}{8}$ 
              [.$\vdots$ ] ] ] ] ]
\end{tikzpicture}
\end{minipage}
\begin{minipage}[b]{.6\linewidth}
\centering
\begin{tikzpicture}[scale=.75,sibling distance=0pt]
\Tree [.$cn$
        [.$\frac{3}{2}cn-c$
          [.$\frac{9}{4}cn-\frac{7}{2}c$
            [.$\frac{27}{8}cn-\frac{37}{4}c$
              [.$\vdots$ ] ] ] ] ] 
\end{tikzpicture}
\end{minipage}
\end{figure}
\end{document}
{% endhighlight %}