---
layout: clrs-solution
title:  "Exercise 4.4-9"
---
>Use a recursion tree to give an asymptotically tight solution to the recurrence $$T(n) = T(\alpha n) +T((1-\alpha)n) + cn$$, where $$\alpha$$ is a constant in the range $$0 < \alpha < 1$$ and $$c > 0$$ is also a constant.

The recurrence $$T(n) = T(\alpha n) + T((1-\alpha)n) + cn$$ has the following recursion tree:

![4.4-9 Recursion Tree]({{ '/assets/img/4-4-9.png' | prepend: site.baseurl }}){:class="latex-img"}

This tree is only complete until level $$\log_{1/(1-\alpha)}n$$. Adding up the costs of each level of the tree:

$$\begin{split}
T(n) &= \sum\limits_{i=0}^{\lg_{1/(1-\alpha)}n} cn \\
& = \left( \sum\limits_{i=1}^{\lg_{1/(1-\alpha)}n} cn \right) + cn \\
& = cn(\log_{1/(1-\alpha)}n) + cn \\
& = \Omega(n\log_{1/(1-\alpha)n}) \\
& = \Omega(n\lg n) \\
\end{split}$$

We guess that $$T(n) \leq bn \lg n$$. Substituting this into the recurrence yields

$$\begin{split}
T(n) & \leq b \alpha n \lg(\alpha n) + b(1-\alpha)n \lg((1-\alpha)n) + cn \\
& = b \alpha n \lg \alpha + b \alpha n \lg n + b(1 - \alpha) n \lg (1 - \alpha) + b(1 - \alpha)n \lg n + cn \\
& = b \alpha n \lg \alpha + b \alpha n \lg n + b(1 - \alpha) n \lg (1 - \alpha) + bn \lg n - b \alpha \lg n + cn \\
& = bn \lg n + bn(\alpha \lg \alpha + (1 - \alpha) \lg(1 - \alpha)) + cn \\
& \leq bn \lg n \\
\end{split}$$

Where the last step holds as long as $$b(\alpha \lg \alpha + (1 - \alpha) \lg (1 - \alpha)) + c \leq 0$$. This bound looks pretty good, so let's guess that our lower bound is $$T(n) \geq bn \lg n$$. Substituting this into the reccurence yields

$$\begin{split}
T(n) & \geq b \alpha n \lg(\alpha n) + b(1-\alpha)n \lg((1-\alpha)n) + cn \\
& = b \alpha n \lg \alpha + b \alpha n \lg n + b(1 - \alpha) n \lg (1 - \alpha) + b(1 - \alpha)n \lg n + cn \\
& = b \alpha n \lg \alpha + b \alpha n \lg n + b(1 - \alpha) n \lg (1 - \alpha) + bn \lg n - b \alpha \lg n + cn \\
& = bn \lg n + bn(\alpha \lg \alpha + (1 - \alpha) \lg(1 - \alpha)) + cn \\
& \geq bn \lg n \\
\end{split}$$

Where the last step holds as long as $$b(\alpha \lg \alpha + (1 - \alpha) \lg (1 - \alpha)) + c \geq 0$$. Therefore $$T(n) = \Theta(n \lg n)$$.

The following LaTeX code was used to generate the above recursion tree:

{% highlight latex %}
\documentclass[12pt]{article}
\usepackage{forest}
\usepackage{tikz-qtree}
\begin{document}

\begin{figure}
\begin{minipage}[b]{0.5\linewidth}
\centering
\begin{tikzpicture}[scale=.75,sibling distance=0pt]
\Tree [.$cn$
        [.$c\alpha n$ 
          [.$c\alpha^2n$ 
            [.$c\alpha^3n$ 
              [.$\vdots$ ] ] 
            [.$c(1-\alpha)\alpha^2n$ 
              [.$\vdots$ ] ] ]
          [.$c(1-\alpha)\alpha n$ 
            [.$c(1-\alpha)\alpha^2n$ 
              [.$\vdots$ ] ] 
            [.$c(1-\alpha)^2\alpha n$ 
              [.$\vdots$ ] ] ] ]
        [.$c(1-\alpha)n$
          [.$c(1-\alpha)\alpha n$ 
            [.$c(1-\alpha)\alpha^2n$ 
              [.$\vdots$ ] ] 
            [.$c(1-\alpha)^2\alpha n$ 
              [.$\vdots$ ] ] ]
          [.$c(1-\alpha)^2n$
            [.$c(1-\alpha)^2\alpha n$ 
              [.$\vdots$ ] ] 
            [.$c(1-\alpha)^3n$ 
              [.$\vdots$ ] ] ] ] ]
\end{tikzpicture}
\end{minipage}
\begin{minipage}[b]{1.1\linewidth}
\centering
\begin{tikzpicture}[scale=.75,sibling distance=0pt]
\Tree [.$cn$
        [.$cn$
          [.$cn$
            [.$cn$
              [.$\vdots$ ] ] ] ] ]
\end{tikzpicture}
\end{minipage}
\end{figure}
\end{document}
{% endhighlight %}