---
layout: clrs-solution
title:  "Exercise 4.6-2"
---
>Show that if $$f(n) = \Theta(n^{\log_b a} \lg^k n)$$, where $$k \geq 0$$, then the master recurrence has solution $$T(n) = \Theta(n^{\log_b a} \lg^{k+1} n)$$. For simplicity, confine your analysis to exact powers of $$b$$.

We have a recurrence of form $$T(n) = aT(n/b) + f(n)$$ which, based on equation 4.21 has the following solution

$$T(n) = \Theta(n^{\log_b a}) + \sum\limits_{j=0}^{\log_{b} n-1} a^j f(n/b^j)$$

Since we have been provided with asymptotic information about $$f(n)$$ let's use that to better define this solution

$$\begin{split}
T(n) & = \Theta(n^{\log_b a}) + \sum\limits_{j=0}^{\log_{b} n-1} a^j \Theta\left((n/b^j)^{\log_b a} \lg^k (n/b^j)\right) \\
& = \Theta(n^{\log_b a}) + \Theta \left( \sum\limits_{j=0}^{\log_{b} n-1} a^j (n/b^j)^{\log_b a} \lg^k (n/b^j)\right) \\
& = \Theta(n^{\log_b a}) + \Theta \left( n^{\log_b a} \sum\limits_{j=0}^{\log_{b} n-1} \left( \frac{a}{b^{\log_b a}} \right)^j \lg^k (n/b^j)\right) \\
& = \Theta(n^{\log_b a}) + \Theta \left( n^{\log_b a} \sum\limits_{j=0}^{\log_{b} n-1} \lg^k (n/b^j)\right) \\
\end{split}$$

Let's pause here for a moment to consider the term trapped by the summation: 

$$\begin{split}
\lg^k(n/b^j) & = ( \lg n - \lg b^j)^k \\
& = \lg^k n - \lg^k b^j \\
\end{split}$$

The right term is troublesome to define, but considering the upper limit of the summation is $$\log_{b} n -1$$ we can deduce that $$\lg^{k}b^j$$ at this upper limit will be $$\lg^k b^{\log_b n - 1} = \lg^k (n-1) < \lg^k{n}$$ which means we can safely remove this term from the summation without impacting the ultimate running time. With this in mind, let's pick up where we left off:

$$\begin{split}
T(n) & = \Theta(n^{\log_b a}) + \Theta \left( n^{\log_b a} \sum\limits_{j=0}^{\log_{b} n-1} \lg^k (n/b^j)\right) \\
& = \Theta(n^{\log_b a}) + \Theta \left( n^{\log_b a} \sum\limits_{j=0}^{\log_{b} n-1} \lg^k n\right) \\
& = \Theta(n^{\log_b a}) + \Theta ( n^{\log_b a} \log_b n \lg^k n) \\
& = \Theta(n^{\log_b a}) + \Theta ( n^{\log_b a} \lg^{k+1} n) \\
& = \Theta ( n^{\log_b a} \lg^{k+1} n) \\
\end{split}$$