---
layout: clrs-solution
title:  "Problem 4-4"
subtitle: "Fibonacci numbers"
---
>This problem develops properties of the Fibonacci numbers, which are defined by the recurrence (3.22). We shall use the technique of generating functions to solve the Fibonacci recurrence. Define the ***generating function*** (or ***formal power series***) $$\mathcal{F}$$ as
>
>$$\begin{split}
\mathcal{F}(z) &= \sum\limits_{i=0}^{\infty} \mathcal{F}_i z^i\\
&= 0 + z + z^2 + 2z^3 + 3z^4 + 5z^5 + 8z^6 + 13z^7 + 21z^8 + \cdots ,\\
\end{split}$$
>
>where $$\mathcal{F}_i$$ is the $$i$$th Fibonacci number.
>
>***a.*** Show that $$\mathcal{F}(z) = z + z\mathcal{F}(z) + z^2 \mathcal{F}(z)$$.

Note that $$\mathcal{f}_i = \mathcal{F}_{i-1} + \mathcal{F}_{i-2} \forall i \geq 2$$, $$\mathcal{F}_{0} = 0$$ and $$\mathcal{F}_{1} = 1$$.

$$\begin{split}
z + z\mathcal{F}(z) + z^2 \mathcal{F}(z) &= z + z \sum\limits_{i=0}^{\infty} \mathcal{F}_i z^i + z^2 \sum\limits_{i=0}^{\infty} \mathcal{F}_i z^i \\
&= z + \sum\limits_{i=1}^{\infty} \mathcal{F}_{i-1} z^i + \sum\limits_{i=0}^{\infty} \mathcal{F}_{i-2} z^i \\
&= z + \mathcal{F}_1 z + \sum\limits_{i=2}^{\infty} (\mathcal{F}_{i-1} + \mathcal{F}_{i-2})z^i \\
&= z + \mathcal{F}_1 z + \sum\limits_{i=2}^{\infty} (\mathcal{F}_{i})z^i \\
&= \sum\limits_{i=0}^{\infty} \mathcal{F}_i z^i \\
&= \mathcal{F}(z) \\
\end{split}$$

>***b.*** Show that 
>
>$$\begin{split}
\mathcal{F}(z) &= \frac{z}{1-z-z^2} \\
&= \frac{z}{(1 - \phi z)(1 - \hat{\phi} z)} \\
&= \frac{1}{\sqrt{5}} \left( \frac{1}{1-\phi z} - \frac{1}{1-\hat{\phi} z} \right), 
\end{split}$$
>
> where
>
>$$\phi = \frac{1 + \sqrt{5}}{2} = 1.61803 \ldots$$
>
>and
>
>$$\hat{\phi} = \frac{1 - \sqrt{5}}{2} = 0.61803 \ldots$$

$$\begin{split}
\mathcal{F}(z) &= \mathcal{F}(z) \left(\frac{1-z-z^2}{1-z-z^2}\right) \\
&= \frac{\mathcal{F}(z) - z \mathcal{F}(z) - z^2 \mathcal{F}(z)}{1 - z - z^2}
\end{split}$$

Let's borrow from question ***a.*** in order to simplify this expression.

$$\begin{split}
&= \frac{\mathcal{F}(z) - (z + z \mathcal{F}(z) + z^2 \mathcal{F}(z)) + z}{1 - z - z^2} \\
&= \frac{\mathcal{F}(z) - \mathcal{F}(z) + z}{1 - z - z^2} \\
&= \frac{z}{1 - z - z^2} \\
\end{split}$$

So far so good. The following identities are helpful in continuing with this problem. $$\phi + \hat{\phi} = \frac{1 + \sqrt{5} + 1 - \sqrt{5}}{2} = 1$$, $$\phi \hat{\phi} = \frac{1 - \sqrt{5} + \sqrt{5} - 5}{2} = -1$$ and $$\phi - \hat{\phi} = \frac{1 + \sqrt{5} - 1 + \sqrt{5}}{2} = \sqrt{5}$$.

$$\begin{split}
&= \frac{z}{1 - (\phi + \hat{\phi})z + \phi \hat{\phi}z^2} \\
&= \frac{z}{(1 - \phi z)(1 - \hat{\phi}z)} \\
&= \frac{\sqrt{5}z}{\sqrt{5}(1 - \phi z)(1 - \hat{\phi}z)} \\
&= \frac{(\phi - \hat{\phi})z + 1 - 1}{\sqrt{5}(1 - \phi z)(1 - \hat{\phi}z)} \\
&= \frac{(1 - \hat{\phi} z) - (1 - \phi z)}{\sqrt{5}(1 - \phi z)(1 - \hat{\phi}z)} \\
&= \frac{1}{\sqrt{5}} \left( \frac{1 - \hat{\phi} z}{(1 - \phi z)(1 - \hat{\phi}z)} - \frac{1 - \phi z}{(1 - \phi z)(1 - \hat{\phi}z)} \right) \\
&= \frac{1}{\sqrt{5}} \left( \frac{1}{1 - \phi z} - \frac{1}{1 - \hat{\phi}z} \right) \\
\end{split}$$

>***c.*** Show that 
>
>$$\mathcal{F}(z) = \sum\limits_{i=0}^{\infty} \frac{1}{\sqrt{5}}(\phi ^i - \hat{\phi^i})z^i$$

For $$\left\lvert x \right\rvert > 1$$ we have $$\frac{1}{1-x} = \sum\limits_{k=0}^{\infty} x ^k$$.

$$\begin{split}
\mathcal{F}(z) &= \frac{1}{\sqrt{5}}\left( \frac{1}{1 - \phi z} - \frac{1}{1 - \hat{\phi} z} \right) \\
&= \frac{1}{\sqrt{5}} \left( \sum\limits_{i=0}^{\infty} (\phi z) ^ i - \sum\limits_{i=0}^{\infty} (\hat{\phi} z)^i \right) \\
&= \frac{1}{\sqrt{5}} \left( \sum\limits_{i=0}^{\infty} \phi ^i z ^ i - \sum\limits_{i=0}^{\infty} \hat{\phi^i} z^i \right) \\
&=  \sum\limits_{i=0}^{\infty} \frac{1}{\sqrt{5}}(\phi ^i z ^ i - \hat{\phi^i} z^i)\\
&=  \sum\limits_{i=0}^{\infty} \frac{1}{\sqrt{5}}(\phi ^i - \hat{\phi^i})z^i \\
\end{split}$$

>***d.*** Use part ***c*** to prove that $$F_i = \frac{\phi^i}{\sqrt{5}}$$ for $$ i > 0$$, rounded to the nearest integer. (*Hint*: Observe that $$\left\lvert \hat{\phi} \right\rvert$$ < 1.)

By this problem's definition and part ***c***, $$F_i = \frac{1}{\sqrt{5}}(\phi ^i - \hat{\phi^i}) = \frac{\phi ^ i}{\sqrt{5}} - \frac{\hat{\phi}^i}{\sqrt{5}}$$. For all values of $$i$$, the subtracted term $$\frac{\hat{\phi}^i}{\sqrt{5}}$$ is less than $$0.5$$ which is therefore effectively rounding the value determined by $$\frac{\phi ^ i}{\sqrt{5}}$$. Thus this problem's popular claim (see SICP 1.13) is simply a restatement of the conclusions of part ***c***.